FreydSSA/Terminator/Extrinsic/Subst.lean
@@ -3,10 +3,11 @@ import FreydSSA.Term.Extrinsic.Subst
 
 variable {φ ν α} [Φ : InstSet φ (Ty α)] [Φc : CohInstSet φ (Ty α)]
 
--- inductive InstSet.USubstL [Φ : InstSet φ (Ty α)] (σ : ν → UTm φ ν)
---   : Ctx ν (Ty α) → LCtx ν κ (Ty α) → Type _
---   | nil : USubstL σ Γ []
---   | cons : USubst σ Γ Δ → USubstL σ Γ L → USubstL σ Γ (sorry :: L)
+inductive InstSet.USubstL [Φ : InstSet φ (Ty α)] (σ : ν → UTm φ ν)
+  : LCtx ν κ (Ty α) → LCtx ν κ (Ty α) → Type _
+  | nil : USubstL σ [] []
+  | cons : USubst σ Γ Δ → USubstL σ L K → USubstL σ (⟨n, A, Γ⟩ :: L) (⟨n, A, Δ⟩ :: K)
+  | skip : USubstL σ L K → ℓ.name ∉ L.labels →  USubstL σ L (ℓ :: K)
 
 -- def UTerminator.Wf.subst {Γ Δ Γ' : Ctx ν (Ty α)} {σ}
 --   {t : UTerminator φ ν κ}
